spec:  w64_to_bytes

proof/spec/Util.ec
@@ -7,17 +7,27 @@ require import BitEncoding.
 from Jasmin require import JModel.
 
 module Util = {
-  proc w64_to_bytes (x : W64.t, outlen : int) = {
-    var r : W8.t list;
-    
-    (* TODO: FIX THIS *)
-    r <- nseq outlen W8.zero;
-  
+  proc w64_to_bytes (in_0 : W64.t, outlen : int) = {
+    var r : W8.t list <- nseq outlen W8.zero;
+    var i : int;
+    var t : W8.t;
+
+    i <- outlen - 1;
+
+    while ((- 1) < i) {
+      t <- (truncateu8 in_0);            (* Get the lowest 8 bits *)
+      r <- put r i t;
+      in_0 <- (in_0 `>>` (W8.of_int 8)); (* Shift right by 8 bits *)
+      i <- i - 1;                        (* Move to the next byte *)
+    }
+
     return r;
   } 
 }.
 
-lemma w64_to_bytes_ll : islossless Util.w64_to_bytes.
+lemma w64_to_bytes_ll : 
+    phoare [Util.w64_to_bytes : 1 < outlen ==> true] = 1%r.
 proof.
+proc.
 admit.
 qed.
